import Relation.Binary.PropositionalEquality as Eq
open Eq using (_≡_; refl; cong; cong-app)
open Eq.≡-Reasoning
open import Data.Nat using (ℕ; zero; suc; _+_)
open import Data.Nat.Properties using (+-comm)

_∘_ : ∀ {A B C : Set} → (B → C) → (A → B) → (A → C)
(g ∘ f) x  = g (f x)

_∘′_ : ∀ {A B C : Set} → (B → C) → (A → B) → (A → C)
g ∘′ f  =  λ x → g (f x)

postulate
  extensionality : ∀ {A B : Set} {f g : A → B}
    → (∀ (x : A) → f x ≡ g x)
      -----------------------
    → f ≡ g

postulate 
  ∀-extensionality : ∀ {A : Set} {B : A → Set} {f g : ∀(x : A) → B x}
    → (∀ (x : A) → f x ≡ g x)
      -----------------------
    → f ≡ g

-- Isomorphism

infix 0 _≃_
record _≃_ (A B : Set) : Set where
  field
    to   : A → B
    from : B → A
    from∘to : ∀ (x : A) → from (to x) ≡ x
    to∘from : ∀ (y : B) → to (from y) ≡ y
open _≃_

≃-refl : ∀ {A : Set}
    -----
  → A ≃ A
≃-refl =
  record
    { to      = λ{x → x}
    ; from    = λ{y → y}
    ; from∘to = λ{x → refl}
    ; to∘from = λ{y → refl}
    }

≃-sym : ∀ {A B : Set}
  → A ≃ B
    -----
  → B ≃ A
≃-sym A≃B =
  record
    { to      = from A≃B
    ; from    = to   A≃B
    ; from∘to = to∘from A≃B
    ; to∘from = from∘to A≃B
    }

≃-trans : ∀ {A B C : Set}
  → A ≃ B
  → B ≃ C
    -----
  → A ≃ C
≃-trans A≃B B≃C =
  record
    { to       = to   B≃C ∘ to   A≃B
    ; from     = from A≃B ∘ from B≃C
    ; from∘to  = λ{x →
        begin
          (from A≃B ∘ from B≃C) ((to B≃C ∘ to A≃B) x)
        ≡⟨⟩
          from A≃B (from B≃C (to B≃C (to A≃B x)))
        ≡⟨ cong (from A≃B) (from∘to B≃C (to A≃B x)) ⟩
          from A≃B (to A≃B x)
        ≡⟨ from∘to A≃B x ⟩
          x
        ∎}
    ; to∘from = λ{y →
        begin
          (to B≃C ∘ to A≃B) ((from A≃B ∘ from B≃C) y)
        ≡⟨⟩
          to B≃C (to A≃B (from A≃B (from B≃C y)))
        ≡⟨ cong (to B≃C) (to∘from A≃B (from B≃C y)) ⟩
          to B≃C (from B≃C y)
        ≡⟨ to∘from B≃C y ⟩
          y
        ∎}
     }

module ≃-Reasoning where

  infix  1 ≃-begin_
  infixr 2 _≃⟨_⟩_
  infix  3 _≃-∎

  ≃-begin_ : ∀ {A B : Set}
    → A ≃ B
      -----
    → A ≃ B
  ≃-begin A≃B = A≃B

  _≃⟨_⟩_ : ∀ (A : Set) {B C : Set}
    → A ≃ B
    → B ≃ C
      -----
    → A ≃ C
  A ≃⟨ A≃B ⟩ B≃C = ≃-trans A≃B B≃C

  _≃-∎ : ∀ (A : Set)
      -----
    → A ≃ A
  A ≃-∎ = ≃-refl

open ≃-Reasoning

infix 0 _≲_
record _≲_ (A B : Set) : Set where
  field
    to      : A → B
    from    : B → A
    from∘to : ∀ (x : A) → from (to x) ≡ x
open _≲_

≲-refl : ∀ {A : Set} → A ≲ A
≲-refl =
  record
    { to      = λ{x → x}
    ; from    = λ{y → y}
    ; from∘to = λ{x → refl}
    }

≲-trans : ∀ {A B C : Set} → A ≲ B → B ≲ C → A ≲ C
≲-trans A≲B B≲C =
  record
    { to      = λ{x → to   B≲C (to   A≲B x)}
    ; from    = λ{y → from A≲B (from B≲C y)}
    ; from∘to = λ{x →
        begin
          from A≲B (from B≲C (to B≲C (to A≲B x)))
        ≡⟨ cong (from A≲B) (from∘to B≲C (to A≲B x)) ⟩
          from A≲B (to A≲B x)
        ≡⟨ from∘to A≲B x ⟩
          x
        ∎}
     }

≲-antisym : ∀ {A B : Set}
  → (A≲B : A ≲ B)
  → (B≲A : B ≲ A)
  → (to A≲B ≡ from B≲A)
  → (from A≲B ≡ to B≲A)
    -------------------
  → A ≃ B
≲-antisym A≲B B≲A to≡from from≡to =
  record
    { to      = to A≲B
    ; from    = from A≲B
    ; from∘to = from∘to A≲B
    ; to∘from = λ{y →
        begin
          to A≲B (from A≲B y)
        ≡⟨ cong (to A≲B) (cong-app from≡to y) ⟩
          to A≲B (to B≲A y)
        ≡⟨ cong-app to≡from (to B≲A y) ⟩
          from B≲A (to B≲A y)
        ≡⟨ from∘to B≲A y ⟩
          y
        ∎}
    }

module ≲-Reasoning where

  infix  1 ≲-begin_
  infixr 2 _≲⟨_⟩_
  infix  3 _≲-∎

  ≲-begin_ : ∀ {A B : Set}
    → A ≲ B
      -----
    → A ≲ B
  ≲-begin A≲B = A≲B

  _≲⟨_⟩_ : ∀ (A : Set) {B C : Set}
    → A ≲ B
    → B ≲ C
      -----
    → A ≲ C
  A ≲⟨ A≲B ⟩ B≲C = ≲-trans A≲B B≲C

  _≲-∎ : ∀ (A : Set)
      -----
    → A ≲ A
  A ≲-∎ = ≲-refl

open ≲-Reasoning

-- Exercise ≃-implies-≲ (practice)

-- Show that every isomorphism implies an embedding. 
-- postulate
≃-implies-≲ : ∀ {A B : Set}
  → A ≃ B
    -----
  → A ≲ B

≃-implies-≲ a≃b =
  record {
    to = to a≃b 
  ; from = from a≃b 
  ; from∘to = from∘to a≃b }


-- Exercise _⇔_ (practice)

-- Define equivalence of propositions (also known as “if and only if”) as follows: 

record _⇔_ (A B : Set) : Set where
  field
    to   : A → B
    from : B → A

-- Show that equivalence is reflexive, symmetric, and transitive.
open _⇔_ -- added

-- This is also an equivalence relation.

⇔-refl : ∀ {A : Set}
    -----
  → A ⇔ A

⇔-refl = record { to = λ x → x ; from = λ x → x }

⇔-sym : ∀ {A B : Set}
  → A ⇔ B
    -----
  → B ⇔ A

⇔-sym A⇔B = record { to = from A⇔B ; from = to A⇔B }

⇔-trans : ∀ {A B C : Set}
  → A ⇔ B
  → B ⇔ C
    -----
  → A ⇔ C

⇔-trans A⇔B B⇔C =
  record {
  to = λ x → to B⇔C (to A⇔B x)
  ; from = λ x → from A⇔B (from B⇔C x) }

-- Recall that Exercises Bin and Bin-laws define a datatype Bin of bitstrings representing
-- natural numbers, and asks you to define the following functions and predicates:

-- to : ℕ → Bin
-- from : Bin → ℕ

-- which satisfy the following property:

-- from (to n) ≡ n
-- Using the above, establish that there is an embedding of ℕ into Bin. 
-- -- Your code goes here

-- Why do to and from not form an isomorphism?
